src/sem/Ptr.v
@@ -2,7 +2,7 @@ From RecordUpdate Require Import RecordSet.
 
 Require SemanticCommon.
 
-Import Addressing Bool Common Condition ExecutionStack Memory MemoryOps Instruction State ZMod
+Import Addressing Bool Common Condition CallStack Memory MemoryOps Instruction State ZMod
   ABI ABI.FatPointer Addressing.Coercions SemanticCommon RecordSetNotations ZArith.
 
 Definition MAX_OFFSET_FOR_ADD_SUB: u256 := int_mod_of _ (2^32)%Z.
