src/sem/Ret.v
@@ -2,7 +2,7 @@ From RecordUpdate Require Import RecordSet.
 
 Require SemanticCommon.
 
-Import Addressing Bool Common Condition ExecutionStack Memory MemoryOps Instruction State ZMod
+Import Addressing Bool Common Condition CallStack Memory MemoryOps Instruction State ZMod
   ABI ABI.Ret ABI.FatPointer Addressing.Coercions SemanticCommon RecordSetNotations.
 (**
 # Returns 
